src/circuit.v
@@ -1,0 +1,4 @@
+From research Require Import base bitvector.
+
+Declare Scope circuit_scope.
+Delimit Scope circuit_scope with circuit.
