src/multiplier2.v
@@ -1,0 +1,288 @@
+(**********************************************************************************)
+(*                                                                                *)
+(*             multiplier2.v - Shift-and-add 4-bit multiplier.                    *)
+(*                                                                                *)
+(*                   +---------------------------+                                *)
+(*                   |                           |                                *)
+(*           A -----------                 ------|------ P                        *)
+(*                   |                           |                                *)
+(*           B -----------        A*B            |                                *)
+(*                   |                           |                                *)
+(*           V -----------                 ------------- R                        *)
+(*                   |                           |                                *)
+(*                   +---------------------------+                                *)
+(*                                                                                *)
+(*  We prove a similiar proof to [multiplier1] except that the circuit has a      *)
+(*  short circuiting mechanism that allows it to end computation early.           *)
+(*  This corresponds to having a more sophisticated predictor function.           *)
+(*                                                                                *)
+(**********************************************************************************)
+
+From research Require Import base bitvector.
+From stdpp Require Import option.
+
+Local Open Scope bv_scope.
+
+Section circuit.
+  Record Registers :=
+    { a : bv 4
+    ; b : bv 4
+    ; c : bv 2
+    ; p : bv 8
+    ; busy : bool
+    }.
+
+  Record _I :=
+    { in_a : bv 4
+    ; in_b : bv 4
+    }.
+
+  Definition I := option _I.
+
+  Record _O :=
+    { out_p : bv 8
+    }.
+
+  Definition O := option _O.
+
+  Definition O0 : O := None.
+
+  Record ILeakage :=
+    { leak_valid : bool
+    ; leak_ready : bool
+    }.
+
+  Record State :=
+    { R : Registers
+    ; T : list ILeakage
+    ; Y : list O
+    }.
+
+  Definition State0 :=
+    {|
+      R := {| a := 0; b := 0; c := 0; p := 0; busy := false |};
+      T := [];
+      Y := []
+    |}.
+
+  Definition shift_and_add (R : Registers) : Registers :=
+    match R.(a) =? 0 with
+    | true => R
+    | false =>
+        let p' : bv 8 :=
+          let t := if R.(a)? then 8#R.(b) else 0 in
+          R.(p) + (t ≪ (8#R.(c)))
+        in
+        let a' := R.(a) ≫ 1 in
+        let c' := R.(c) + 1 in
+        R <| a := a' |> <| p := p' |> <| c := c' |>
+    end.
+
+  Definition circuit_step (s : State) (x : I) : State :=
+    match s.(R).(busy) with
+    | false =>
+        match x with
+        | Some x =>
+            let R' := {| a := x.(in_a); b := x.(in_b); c := 0; p := 0; busy := true |} in
+            let T' := s.(T) ++ [{| leak_valid := true; leak_ready := false |}] in
+            let Y' := s.(Y) ++ [None] in
+            s <| R := R' |> <| T := T' |> <| Y := Y' |>
+        | None =>
+            let T' := s.(T) ++ [{| leak_valid := false; leak_ready := false |}] in
+            let Y' := s.(Y) ++ [None] in
+            s <| T := T' |> <| Y := Y' |>
+        end
+    | true =>
+        let leak_valid' := match x with Some _ => true | _ => false end in
+        match s.(R).(a) =? 0 with
+        | true =>
+            let R' := s.(R) <| busy := false |> in
+            let T' := s.(T) ++ [{| leak_valid := leak_valid'; leak_ready := true |}] in
+            let Y' := s.(Y) ++ [Some {| out_p := s.(R).(p) |}] in
+            s <| R := R' |> <| T := T' |> <| Y := Y' |>
+        | false =>
+            let R' := shift_and_add s.(R) in
+            let T' := s.(T) ++ [{| leak_valid := leak_valid'; leak_ready := false |}] in
+            let Y' := s.(Y) ++ [None] in
+            s <| R := R' |> <| T := T' |> <| Y := Y' |>
+        end
+    end.
+
+  Definition circuit_steps s xs := fold_left circuit_step xs s.
+
+  Compute (
+      circuit_steps State0
+        [Some {| in_a := 14; in_b := 14 |}; None; None; None; None; None]
+    ).
+End circuit.
+
+Section ct.
+  Record _SLeakage := { leak_a : bv 4 }.
+  Definition SLeakage := option _SLeakage.
+
+  Definition public1 : I -> SLeakage :=
+    option_map (fun x => {| leak_a := x.(in_a) |}).
+
+  Definition public := map public1.
+
+  Definition PredictorState := option (bv 4).
+
+  Definition predictor_step (st : PredictorState) (s : SLeakage) :=
+    match st with
+    | Some x =>
+        match x =? 0 with
+        | true => None
+        | false => Some (x ≫ 1)
+        end
+    | None =>
+        match s with
+        | Some {| leak_a := x |} => Some x
+        | None   => None
+        end
+    end.
+
+  Definition predictor_steps (st : PredictorState) (xs : list SLeakage) :=
+    fold_left predictor_step xs st.
+
+  Definition predict_next (st : PredictorState) (s : SLeakage) :=
+    match st with
+    | Some x =>
+        let leak_valid' := match s with Some _ => true | None => false end in
+        let leak_ready' := x =? 0 in
+        {| leak_valid := leak_valid'; leak_ready := leak_ready' |}
+    | None =>
+        match s with
+        | Some _ => {| leak_valid := true; leak_ready := false |}
+        | None => {| leak_valid := false; leak_ready := false |}
+        end
+    end.
+
+  Fixpoint predict' st xs :=
+    match xs with
+    | [] => []
+    | x :: xs' => predict_next st x :: predict' (predictor_step st x) xs'
+    end.
+
+  Definition predict xs := predict' None xs.
+
+  Definition rep (x : State) (y : PredictorState) : Prop :=
+    (exists v, y = Some v /\ x.(R).(a) = v /\ x.(R).(busy) = true)
+    \/ (y = None /\ x.(R).(busy) = false).
+
+  Infix "`R`" := rep (at level 70).
+
+  Lemma simulation_step : forall s1 s2 s1' s2' x,
+      s1 `R` s2 ->
+      s1' = circuit_step s1 x ->
+      s2' = predictor_step s2 (public1 x) ->
+      s1' `R` s2'.
+  Proof.
+    unfold rep, circuit_step, predictor_step, public1, option_map.
+    simplify. inv H.
+    - inv H0 as [v]. propositional. rewrite H2. simplify.
+      destruct (s1.(R).(a) =? 0) eqn:Heqn; simplify.
+      + eauto.
+      + left. exists (s1.(R).(a) ≫ 1). propositional.
+        * unfold shift_and_add. rewrite Heqn. simplify.
+          equality.
+        * unfold shift_and_add. rewrite Heqn. simplify.
+          equality.
+    - inv H0. rewrite H1. simplify. destruct x as [x'|]; simplify.
+      + left. exists (x'.(in_a)). equality.
+      + right. equality.
+  Qed.
+
+  Lemma simulation_initial : State0 `R` None.
+  Proof. unfold rep; equality. Qed.
+
+  Lemma simulation_many_step : forall xs s1 s2 s1' s2',
+    s1 `R` s2 ->
+    s1' = circuit_steps s1 xs ->
+    s2' = predictor_steps s2 (public xs) ->
+    s1' `R` s2'.
+  Proof.
+    induction xs as [| y ys IHy ]; simplify; try equality.
+    - assert (rep (circuit_step s1 y) (predictor_step s2 (public1 y))).
+      { apply simulation_step with (s1 := s1) (s2 := s2) (x := y); eauto. }
+      unfold circuit_steps, predictor_steps. eapply IHy; eauto.
+  Qed.
+
+  Definition leak_next (s : State) (x : I) :=
+    match s with
+    | {| R := {| a := a; busy := true |} |} =>
+        let leak_valid' := match x with Some _ => true | None => false end in
+        let leak_ready' := a =? 0 in
+        {| leak_valid := leak_valid'; leak_ready := leak_ready' |}
+    | {| R := {| busy := false |} |} =>
+        match x with
+        | Some _ => {| leak_valid := true; leak_ready := false |}
+        | None => {| leak_valid := false; leak_ready := false |}
+        end
+    end.
+
+  Lemma simulation_predict_leak : forall s1 s2 x,
+      s1 `R` s2 -> leak_next s1 x = predict_next s2 (public1 x).
+  Proof.
+    unfold rep, leak_next, predict_next, public1.
+    simplify. inv H.
+    - firstorder; simplify. destruct s1; simplify.
+      destruct R0; simplify. unfold option_map; simplify.
+      destruct x; eauto.
+    - propositional; simplify. destruct s1; simplify.
+      destruct R0; simplify. unfold option_map; simplify.
+      destruct x; eauto.
+  Qed.
+
+  Lemma predict_app' : forall xs ys1 ys2 x s,
+      ys1 = predict' s xs ->
+      ys2 = predict' s (xs ++ [x]) ->
+      ys2 = ys1 ++ [predict_next (predictor_steps s xs) x].
+  Proof.
+    induction xs as [| z zs IHz ]; simplify.
+    - equality.
+    - f_equal. apply IHz; equality.
+  Qed.
+
+  Lemma predict_app : forall xs x,
+      predict (xs ++ [x]) =
+        predict xs ++ [predict_next (predictor_steps None xs) x].
+  Proof.
+    simplify. apply predict_app'; equality.
+  Qed.
+
+  Lemma circuit_steps_app' : forall xs x s1 s2 s3,
+      s2 = circuit_steps s1 xs ->
+      s3 = circuit_steps s1 (xs ++ [x]) ->
+      s3.(T) = s2.(T) ++ [leak_next s2 x].
+  Proof.
+    induction xs as [| z zs IHz ]; simplify.
+    - unfold circuit_step, leak_next.
+      destruct s1 as [R T Y]. destruct R as [a b count busy].
+      simplify. repeat case_match; simplify_bv_eqb; simplify; eauto.
+      all: try rewrite H0; eauto.
+    - apply IHz with (s1 := (circuit_step s1 z)); equality.
+  Qed.
+
+
+  Lemma circuit_steps_app : forall xs x,
+      T (circuit_steps State0 (xs ++ [x])) =
+        T (circuit_steps State0 xs) ++ [leak_next (circuit_steps State0 xs) x].
+  Proof.
+    simplify. apply circuit_steps_app' with (xs := xs) (s1 := State0); equality.
+  Qed.
+
+  Theorem circuit_ct : exists f, forall xs s,
+      s = circuit_steps State0 xs -> s.(T) = f (public xs).
+  Proof.
+    exists predict.
+    induction xs as [| z zs IHz ] using rev_ind; simplify.
+    - equality.
+    - rewrite circuit_steps_app. unfold public. rewrite map_app.
+      simplify. rewrite predict_app. rewrite IHz by equality.
+      unfold public. repeat f_equal. apply simulation_predict_leak.
+      apply simulation_many_step with (xs := zs) (s1 := State0) (s2 := None).
+      + apply simulation_initial.
+      + equality.
+      + equality.
+  Qed.
+End ct.
