Makefile
@@ -35,10 +35,12 @@ endif
 	@rocq c $(COQARGS) $(shell cat '_CoqProject') $< -o $@
 
 clean:
-	@echo "CLEAN vo glob aux"
-	@rm -f $(ALL_VFILES:.v=.vo) $(ALL_VFILES:.v=.glob)
+	@echo "CLEAN vo glob vok vos aux cache"
+	@rm -f $(ALL_VFILES:.v=.vo) $(ALL_VFILES:.v=.glob) $(ALL_VFILES:.v=.vok) $(ALL_VFILES:.v=.vos)
 	@find $(SRC_DIRS) -name ".*.aux" -exec rm {} \;
 	rm -f _CoqProject .coqdeps.d
+	@rm -f .nia.cache .lia.cache
+	@find $(SRC_DIRS) -name ".*.cache" -exec rm {} \;
 
 .PHONY: default test clean
 .DELETE_ON_ERROR:
